

1. Let X be a normed linear space and $\varphi_1, \varphi_2, \dots, \varphi_n, n \in \mathbb{N}$, be linearly independent vectors in X' . Show that there exist $x_1, x_2, \dots, x_n \in X$ such that

$$\varphi_i(x_j) = \delta_{ij} := \begin{cases} 1 & i = j \\ 0 & i \neq j \end{cases} \quad 1 \leq i, j \leq n.$$

(Compare this problem with Problem 4 in Homework 1)

Let $Y = \text{span}\{\varphi_i\} \subseteq X'$, $\varphi = \sum_{i=1}^n a_i \varphi_i$
 Let ℓ_i be from the canonical mapping of $X \rightarrow X''$
 $\ell_i: Y' \rightarrow \mathbb{C} \quad \varphi \mapsto \varphi(x_i)$

We also know from a lemma in class that each ℓ_i is well defined and the canonical mapping is injective. Since the mapping is injective, $\exists \{x_i\} \in X \exists C(x_i) = \ell_i$ for each φ_i as ℓ_i is determined by actions on L.T. φ_i .

Let $Y = \text{span}\{x_i\}$ and $y = \sum_{j=1}^n b_j x_j$
 $\varphi(y) = \sum_{i=1}^n a_i \varphi_i(y) = \varphi(\sum_{j=1}^n b_j x_j) = \sum_{j=1}^n b_j \varphi(x_j)$

$$\text{Thus } a_i = \varphi(x_i) \text{ and } b_j = \varphi_j(y) \\ \Rightarrow \varphi(x_j) = \sum_{i=1}^n a_i \varphi_i(x_j) = \sum_{i=1}^n \varphi(x_i) \varphi_i(x_j) \Rightarrow \varphi_i(x_j) = \delta_{ij}$$

2. Consider the operator $T: l^1 \rightarrow l^1$ defined by

$$T(\{x_1, \dots, x_n, \dots\}) = (\{0, x_1, x_2, \dots, x_n, \dots\}), \quad \forall \{x_n\} \in l^1.$$

Show that $T \in \mathcal{B}(l^1, l^1)$ and find T^* .

$$\text{Let } x \in l^1 \quad \|x\| = \sum_{i=1}^{\infty} |x_i| = 0 + \sum_{i=2}^{\infty} |x_{i-1}| = \|Tx\|$$

$$\text{Thus } T \in \mathcal{B}(l^1, l^1)$$

$$T^* g x = g T x$$

Note $(l^1)' \cong l^\infty$ Thus $g \in l^\infty$

$$g T x = \sum_{i=1}^{\infty} |g_{i+1} x_i| = \sum_{i=2}^{\infty} |g_i x_{i-1}| = T^* g x$$

Thus $T^*: Y' \rightarrow X'$ $g \mapsto \{g_2, g_3, \dots\}$ (left shift)

3. Let X, Y be normed linear spaces and $T \in \mathcal{B}(X, Y)$. Show that if T^{-1} exists and $T^{-1} \in \mathcal{B}(Y, X)$, then $(T^*)^{-1}$ also exists and $(T^*)^{-1} = (T^{-1})^*$.

Since T^{-1} exists T is bijective.

$T^{-1} \in \mathcal{B}(Y, X)$, then $(T^*)^{-1}$ also exists and $(T^*)^{-1} = (T^{-1})^*$.

Since T^{-1} exists, T is bijective.

Let $\varphi_y \in N(T^*)$ and $x \in X$

$0 = T^* \varphi_y x = \varphi_y T x \Rightarrow \varphi_y = 0$ since T is injective and x was arbitrary

Thus T^* is injective

Let $\varphi_x \in X'$ WTS $\exists \varphi_y \in Y' \ni T^* \varphi_y = \varphi_x$

Let $x \in X$

Define $\varphi_y := \varphi_x T^{-1}$

$$T^* \varphi_y x = \varphi_y T x = \varphi_x T^{-1} T x = \varphi_x x$$

Thus T^* is surjective.

$\exists T^*$ is a bijection $\Rightarrow \exists (T^*)^{-1}$

$$\text{WTS } (T^*)^{-1} = (T^{-1})^*$$

Let $\varphi \in X'$ $x \in X$ $\varphi_y \in Y'$ $y \in Y$

$$\text{Consider } T^* (T^{-1})^* \varphi x = T^* \varphi T^{-1} x = \varphi T T^{-1} x = \varphi x$$

$$\text{Similarly } (T^{-1})^* T^* \varphi_y y = (T^{-1})^* \varphi_y T y = \varphi_y T^{-1} T y = \varphi_y y$$

$$\therefore (T^{-1})^* T^* = I_Y \text{ and } T^* (T^{-1})^* = I_X \Rightarrow (T^{-1})^* = (T^*)^{-1}$$

4. Recall the space $C^1[0, 1]$ defined by

$$C^1[0, 1] := \{f \in C[0, 1] : f' \text{ exists and } f' \text{ is continuous on } [0, 1]\}$$

is a Banach space with the norm

$$\|f\|_{C^1} := \max_{x \in [0, 1]} |f(x)| + \max_{x \in [0, 1]} |f'(x)|.$$

(a) Show that for each $x \in [0, 1]$, the functional $\varphi_x : C^1[0, 1] \rightarrow \mathbb{R}$, defined by

$$\varphi_x(f) := f'(x)$$

is a bounded linear functional on $(C^1[0, 1], \|\cdot\|_{C^1})$.

(b) Fix $g : [0, 1] \rightarrow [0, 1]$ in $C^1[0, 1]$ and define T_g on $C^1[0, 1]$ by $T_g(f) = f \circ g$. Show that T_g is a bounded linear operator on $C^1[0, 1]$ and find $T_g^*(\varphi_x)$.

a) Let $f_1, f_2 \in C'$ $\alpha \in \mathbb{R}$

a) Let $f_1, f_2 \in C'$ $\alpha \in \mathbb{R}$

$$\varphi_x(\alpha f_1 + f_2) = \frac{d}{dx}[\alpha f_1(x) + f_2(x)] = \alpha f_1'(x) + f_2'(x) = \alpha \varphi_x(f_1) + \varphi_x(f_2)$$

$$|\varphi_x f| = |f'(x)| \leq \max_{x \in X} |f'(x)| \leq \|f\|_{C'}$$

b) Let $f_1, f_2 \in C'$ $\alpha \in \mathbb{R}$

$$T_g(\alpha f_1 + f_2) = (\alpha f_1 + f_2) \circ g = \alpha f_1 \circ g + f_2 \circ g = \alpha T_g(f_1) + T_g(f_2)$$

$$|T_g f| = |f(g(x))| \leq \max_{x \in X} |f(x)| \leq \|f\|_{C'}$$

WTF $T_g^*(\varphi_x)$

$$T_g^* \varphi_x f = \varphi_x T_g f = \varphi_x f(g(x)) = f'(g(x)) g'(x)$$

$$\text{Thus } T_g^* \varphi_x f = f'(g(x)) g'(x)$$

5. Show that every Hilbert space is reflexive.

WTS \mathcal{C} is surjective
 $\Rightarrow \mathcal{C}H = H''$

Define $A: H' \rightarrow H$ $f \mapsto z$

Where x is the Riesz representative of f .

Notice for $\alpha, \beta \in \mathbb{C}$ $f_1, f_2 \in H'$

$$(\alpha f_1 + \beta f_2)x = \alpha f_1(x) + \beta f_2(x) = \alpha \langle x, z_1 \rangle + \beta \langle x, z_2 \rangle$$

$$\text{Thus } A(\alpha f_1 + \beta f_2) = \bar{\alpha} A f_1 + \bar{\beta} A f_2 = \langle x, \bar{\alpha} z_1 + \bar{\beta} z_2 \rangle$$

Define $\langle f, g \rangle_1 = \langle A g, A f \rangle$

$$\begin{aligned} \langle x+y, h \rangle_1 &= \langle A h, A(x+y) \rangle \\ &= \langle A h, A x \rangle + \langle A h, A y \rangle \\ &= \langle x, h \rangle_1 + \langle y, h \rangle_1 \end{aligned}$$

$$\langle x, y \rangle_1 = \langle A y, A x \rangle = \overline{\langle A x, A y \rangle} = \overline{\langle y, x \rangle_1}$$

$$\langle x, x \rangle_1 = 0 = \langle A x, A x \rangle \Rightarrow A x = 0 \Rightarrow x = 0$$

$$\langle \alpha x, y \rangle_1 = \langle A y, A \alpha x \rangle = \langle A y, \bar{\alpha} A x \rangle = \alpha \langle A y, A x \rangle = \alpha \langle x, y \rangle_1$$

H' is complete as \mathbb{C} is complete.
 Thus $(H', \langle \cdot, \cdot \rangle_1)$ is a Hilbert space.

$$\text{Let } g \in H'' \text{ and } g(f) = \langle f, f_0 \rangle_1 = \langle A f_0, A f \rangle = \langle A f_0, z \rangle = f(A f_0)$$

Let $g \in H''$ and $g(F) = \underset{\text{RFT}}{\langle f, f_0 \rangle} = \langle Af_0, Af \rangle = \langle Af_0, z \rangle = f(Af_0)$
 Thus $g = CAf_0$ where C is the canonical mapping.

$\therefore C$ is surjective $\Rightarrow H \cong H''$

6. Let X be a normed linear space. Show that if X is reflexive, then for any $\varphi \in X'$, there exists $x \in X$ with $\|x\| = 1$ such that $\|\varphi\| = \varphi(x)$.

Since X is reflexive, $X'' \cong X$ or the dual of X' is isomorphic to X .

If $\varphi = 0 \quad \forall x \in X \exists \|x\|=1 \wedge \|\varphi\|=0=\varphi(x)$

By a corollary of H-B $\forall \varphi \in X' \setminus \{0\} \exists l_x \in X'' \exists \|l_x\|=1$ and $l_x \varphi = \|\varphi\|$.

Since X is reflexive $\forall l_x \in X'' \exists x \in X \exists \|l_x\|=\|x\|$ and $l_x \varphi = \varphi(x)$

Thus $\exists x \in X \exists \|x\|=1$ and $\varphi(x) = \|\varphi\|$

7. Show that a Banach space X is reflexive if and only if its dual space X' is reflexive.

(\Rightarrow) WTS $(X^*)^{**} \cong X^*$

Given $X^{**} \cong X$

We can write $(X^*)^{**} = (X^{**})^* \cong (X)^*$

thus X^* is reflexive.

(\Leftarrow) WTS $X \cong X^{**}$ Given $X^* \cong (X^*)^{**}$

Let $l_x \in X^{**} \quad \psi \in X^{***} \quad \varphi \in X^* \exists C, \varphi = C\psi$

$\psi l_x = l_x \psi = \varphi(x) \Rightarrow \exists x \in X \exists C x = l_x$

$\therefore C$ is surjective $\Rightarrow X \cong X^{**}$

.. \cup is subjective -/ $\lambda = \lambda''$